# 2次関数

## 解の公式の証明

\\[
    ax^2+bx+c=0 \\\\
    a\left(x^2+\frac{b}{a}x+\left(\frac{b}{2a}\right)^2-\left(\frac{b}{2a}\right)^2\right)+c=0 \\\\
    a\left(x+\frac{b}{2a}\right)^2-\frac{b^2}{4a}+c=0 \\\\
    a\left(x+\frac{b}{2a}\right)^2=\frac{b^2}{4a}-c \\\\
    a\left(x+\frac{b}{2a}\right)^2=\frac{b^2-4ac}{4a} \\\\
    \left(x+\frac{b}{2a}\right)^2=\frac{b^2-4ac}{4a^2} \\\\
    x+\frac{b}{2a}=\pm{\sqrt{\frac{b^2-4ac}{4a^2}}} \\\\
    x+\frac{b}{2a}=\pm{\frac{\sqrt{b^2-4ac}}{2a}} \\\\
    x={\frac{-b\pm\sqrt{b^2-4a^2c}}{2a}} \\\\
\\]